Reduce amount of stability obligations, work on example

Core/Linearizability.v
@@ -11,6 +11,7 @@ From LHL.Core Require Import
 
 From Coq Require Import
   Lists.List.
+Import ListNotations.
 
 Definition KConc {E} (spec : Spec E) : Spec E := overObj (spec :> idImpl).
 
@@ -20,9 +21,10 @@ Definition Lin {E} (spec' : Spec E) (spec : Spec E) :=
 Definition HBRw_ {E} (evs evs' : Trace (ThreadEvent E)) : Prop :=
     exists h h' i i' m m',
       i <> i' /\
-      evs = h ++ (cons (i, m) (cons (i', m') nil)) ++ h' /\
-      ((exists Ret (e : E Ret), m = CallEv e) \/ (exists Ret (e : E Ret) (v : Ret), m' = RetEv e v)) /\
-      evs' = h ++ (cons (i', m') (cons (i, m) nil)) ++ h'.
+      evs = h ++ [(i, m); (i', m')] ++ h' /\
+      ((exists Ret e, m = @CallEv E Ret e) \/
+       (exists Ret e v, m' = @RetEv E Ret e v)) /\
+      evs' = h ++ [(i', m'); (i, m)] ++ h'.
 
 Definition HBRw {E} : (Trace (ThreadEvent E)) -> (Trace (ThreadEvent E)) -> Prop :=
   clos_refl_trans (Trace (ThreadEvent E)) HBRw_.
@@ -42,15 +44,7 @@ Inductive AllCallEv {E} : Trace (@ThreadEvent E) -> Prop :=
 Definition LinRw {E} : 
   (Trace (ThreadEvent E)) -> (Trace (ThreadEvent E)) -> Prop :=
   fun s t => exists sO sP, 
-    AllCallEv sO /\ AllRetEv sP /\ 
+    AllRetEv sP /\ AllCallEv sO /\
     HBRw (s ++ sP) (t ++ sO).
 
 Notation LinToSpec ρ V := (exists l, IsTraceOfSpec l V /\ LinRw ρ l). 
-
-Definition lin {E} (V : Spec E) (ρ : Trace (ThreadEvent E)) : Trace (ThreadEvent E).
-Admitted.
-
-Lemma lin_correct {E} {V : Spec E} ρ :
-  let σ := lin V ρ in
-  LinToSpec σ V /\ forall ρ', LinToSpec ρ' V -> PrefixOf ρ' ρ -> PrefixOf ρ' σ.
-Admitted.
