Examples/AtomicCounter.v
@@ -7,12 +7,16 @@ From LHL.Core Require Import
   Traces
   Linearizability.
 
+From LHL.Util Require Import
+  TransUtil.
+
 From LHL.Examples Require Import
   RacyCounter
   CounterSpecs
   Lock.
 
 From Coq Require Import
+  Arith.PeanoNat
   Program.Equality
   Lists.List
   Relations.Relation_Operators.
@@ -53,6 +57,137 @@ Definition VF := atomicCounterSpec.
 
 Definition Relt := Relt E VE F.
 Definition Prec := Prec E VE F.
+Definition Post := Post E VE F.
+
+Inductive Atomic : Trace (ThreadEvent F) -> Prop :=
+| NilAtomic : Atomic []
+| ConsAtomic {i ρ A} {m : F A} {v : A} :
+  Atomic ρ ->
+  Atomic ((i, CallEv m) :: (i, RetEv m v) :: ρ).
+
+Lemma decideEqNat : forall (n m : nat), {n = m} + {n <> m}.
+fix rec 2.
+intros.
+destruct n, m.
+left.
+congruence.
+right.
+congruence.
+right.
+congruence.
+assert ({n = m} + {n <> m}) by apply rec.
+destruct H.
+left.
+congruence.
+right.
+congruence.
+Qed.
+
+Lemma decideAtomic : forall ρ, {Atomic ρ} + {~(Atomic ρ)}.
+fix rec 1.
+intros.
+destruct ρ.
+left.
+constructor.
+destruct ρ.
+right.
+unfold not.
+intros.
+inversion H.
+destruct t, t0.
+assert ({t = t0} + {t <> t0}) by apply decideEqNat.
+destruct H.
+subst.
+{
+  destruct e, e0.
+  right.
+  unfold not.
+  intros.
+  inversion H.
+  {
+    destruct m, m0.
+    assert ({Atomic ρ} + {~Atomic ρ}) by apply rec.
+    destruct H.
+    left.
+    constructor.
+    easy.
+    right.
+    unfold not.
+    intros.
+    apply n0.
+    inversion H.
+    easy.
+    right.
+    unfold not.
+    intros.
+    dependent destruction H.
+    right.
+    unfold not.
+    intros.
+    dependent destruction H.
+    assert ({Atomic ρ} + {~Atomic ρ}) by apply rec.
+    destruct H.
+    left.
+    constructor.
+    easy.
+    right.
+    unfold not.
+    intros.
+    dependent destruction H.
+    apply n0.
+    easy.
+  }
+  right.
+  unfold not.
+  intros.
+  inversion H.
+  right.
+  unfold not.
+  intros.
+  inversion H.
+}
+right.
+unfold not.
+intros.
+inversion H.
+congruence.
+Qed.
+
+Definition AtomicPrefix (ρ σ : Trace (ThreadEvent F)) : Prop :=
+  exists τ,
+    σ = ρ ++ τ /\
+    Atomic ρ /\
+    ~(Atomic τ).
+
+(*
+left = atomic   right = nonatomic
+acc should always be atomic
+*)
+Fixpoint linAux (acc ρ : Trace (ThreadEvent F)) : Trace (ThreadEvent F) :=
+  match ρ with
+  | [] | [_] => acc
+  | e1 :: e2 :: σ =>
+    match decideAtomic (acc ++ [e1; e2]) with
+    | left _ => linAux (acc ++ [e1; e2]) σ
+    | right _ => acc
+    end
+  end.
+
+Definition lin ρ := linAux [] ρ.
+
+Lemma linSplit ρ σ :
+  ~Atomic σ ->
+  lin (ρ ++ σ) = lin ρ.
+Admitted.
+
+Lemma linSat ρ :
+  lin (lin ρ) = lin ρ.
+Admitted.
+
+Lemma linAtomic ρ :
+  Atomic ρ ->
+  lin ρ = ρ.
+Admitted.
 
 Definition countState (s : @InterState E F VE) : RacyCounterState :=
   snd (snd s).
@@ -60,109 +195,225 @@ Definition countState (s : @InterState E F VE) : RacyCounterState :=
 Definition lockState (s : @InterState E F VE) : LockState :=
   fst (snd s).
 
-Definition int i : Relt :=
+Definition AtomicCounterSteps :
+  AtomicCounterState -> Trace (ThreadEvent CounterSig) -> AtomicCounterState -> Prop :=
+  Steps AtomicCounterStep.
+
+Lemma atomicTrans m :
+  forall ρ n,
+  AtomicCounterSteps (CounterIdle n) ρ (CounterIdle m) ->
+  Atomic ρ.
+fix rec 1.
+intros.
+destruct ρ.
+constructor.
+destruct ρ.
+dependent destruction H.
+dependent destruction H.
+dependent destruction H0.
+dependent destruction H0.
+do 2 dependent destruction H.
+dependent destruction H0.
+dependent destruction H.
+constructor.
+eapply rec.
+exact H0.
+dependent destruction H0.
+dependent destruction H.
+constructor.
+eapply rec.
+exact H0.
+Qed.
+
+Definition inter i : Relt :=
   fun s ρ t σ =>
-    InvokeAny atomicCounterImpl i s ρ t σ \/
-    ReturnAny atomicCounterImpl i s ρ t σ.
+    exists j,
+      j <> i /\
+      ((InvokeAny atomicCounterImpl j s ρ t σ) \/
+        ReturnAny atomicCounterImpl j s ρ t σ).
+
 
 Definition rely : ThreadName -> Relt :=
   fun i s ρ t σ =>
-      RTC
-        (fun s ρ t σ => exists j, i <> j /\ int j s ρ t σ)
-        s ρ t σ \/
+      inter i s ρ t σ \/
       (lockState s = LockOwned i ->
         countState s = countState t /\
-        lin VF ρ = lin VF σ /\
-        lockState t = LockOwned i).
+        lin ρ = lin σ).
+
+Lemma relyTrans i :
+  rely i >> rely i ==> rely i.
+unfold rely, inter, sub, subRelt, InvokeAny, TInvoke, ReturnAny, TReturn.
+intros.
+psimpl.
+destruct H, H0.
+psimpl.
+destruct H2, H1.
+{
+  psimpl.
+}
+Admitted.
 
 Definition guar : ThreadName -> Relt :=
   fun i s ρ t σ =>
-      RTC (int i) s ρ t σ \/
-      (lockState s <> LockOwned i ->
+      lockState s <> LockOwned i ->
         countState s = countState t /\
-        lin VF ρ = lin VF σ).
+        lin ρ = lin σ.
+
+Definition invariant i (f : nat -> AtomicCounterState) : Prec :=
+  fun s ρ =>
+    exists k (b : bool),
+      countState s = CounterDSt (f k) /\
+      AtomicCounterSteps
+        (CounterIdle 0)
+        (lin ρ ++
+          if b then
+            [(i, CallEv Inc)]
+          else
+            [])
+        (f k).
 
 Definition precs : ThreadName -> forall Ret, CounterSig Ret -> Prec :=
   fun i Ret m s ρ =>
     TIdle i s ρ /\
-    countState s <> CounterUB /\
+    invariant i CounterIdle s ρ /\
     lockState s <> LockOwned i.
 
-Definition posts : ThreadName -> forall Ret, CounterSig Ret -> Relt :=
-  fun i Ret m s ρ t σ =>
-    lockState s <> LockOwned i /\
-    exists n,
-    countState s = CounterDSt (CounterIdle n) /\
-    match m with
-    | Get => True
-    | Inc => countState t = CounterDSt (CounterIdle (S n))
-    end.
+Definition posts : ThreadName -> forall Ret, CounterSig Ret -> Post Ret :=
+  fun i Ret m v _ _ t σ =>
+    invariant i CounterIdle t σ /\
+    lockState t <> LockOwned i.
+
+Ltac rw_all :=
+repeat match goal with
+| [ H : ?x = ?y |- ?G ] => try (rewrite H in *); clear H
+end.
+
+Ltac commit :=
+unfold Commit, precs, guar, invariant, countState, lockState;
+intros;
+psimpl.
+
+Lemma listHelpAbsurd {A} {xs ys : list A} {x : A} :
+  [] <> xs ++ x :: ys.
+Admitted.
 
 Theorem atomicCounterCorrect :
   VerifyImpl VE VF rely guar precs atomicCounterImpl posts.
 unfold VerifyImpl.
 split.
-intros.
 {
-  unfold sub, subRelt.
+  unfold guar, rely, sub, subRelt.
   intros.
-  pdestruct H.
-  destruct H, H0.
-  left.
-  apply rtcTrans.
-  psplit.
-  exact H.
-  easy.
-  left.
-  admit.
   right.
   intros.
-  apply H in H1.
-  clear H.
-  do 2 destruct H1.
-  apply H0 in H2.
-  clear H0.
-  do 2 destruct H2.
-  split.
-  etransitivity.
-  exact H.
-  easy.
-  split.
-  etransitivity.
-  exact H1.
-  easy.
-  easy.
+  apply H0.
+  congruence.
 }
-split.
-admit.
-split.
-admit.
-split.
-admit.
 split.
 admit.
 split.
 admit.
 intros.
 destruct m.
+simpl.
+unfold inc.
 {
-  simpl.
-  unfold inc.
-  eapply weakenPost.
-  eapply safeBindUnit with
+  eapply safeBind with
     (QI:= fun s ρ t σ =>
-      countState t <> CounterUB /\
+      invariant i CounterIdle t σ /\
       lockState t <> LockOwned i)
     (QR:= fun s ρ t σ =>
-      countState t <> CounterUB /\
-      lockState t = LockOwned i).
+      lockState s <> LockOwned i /\
+      lockState t = LockOwned i /\
+      countState s = countState t /\
+      ρ = σ /\
+      invariant i CounterIdle t σ).
   {
-    stable.
-    unfold Stable, stablePrec, sub, subPrec, precs, rely.
-    intros.
-    pdestruct H.
+    admit.
   }
   {
-    unfold Stable
+    commit.
+    dependent destruction H11.
+    destruct x2.
+    admit.
+    eexists.
+    split.
+    split.
+    exists x1, false.
+    split.
+    congruence.
+    exact H5.
+    congruence.
+    split.
+    intros.
+    split.
+    easy.
+    rewrite linSplit.
+    easy.
+    unfold not.
+    intros.
+    dependent destruction H11.
+    exists [].
+    split.
+    constructor.
+    exists [(i, CallEv Inc)], [].
+    constructor.
+    constructor.
+    constructor.
+    split.
+    constructor.
+    do 2 rewrite app_nil_r.
+    apply rt_refl.
+  }
+  admit.
+  split.
+  {
+    commit.
+    dependent destruction H6.
+    eexists.
+    split.
+    split.
+    congruence.
+    split.
+    congruence.
+    split.
+    easy.
+    split.
+    easy.
+    exists x2, false.
+  }
+  eapply safeBind with
+    (QI:= fun s ρ t σ =>
+      invariant (fun k => CounterIncRunning k i) t σ /\
+      lockState t = LockOwned i)
+    (QR:= fun s ρ t σ =>
+      lockState s = LockOwned i /\
+      invariant CounterIdle t σ).
+  admit.
+  {
+    commit.
+    dependent destruction H5.
+    congruence.
+    dependent destruction H5.
+    eexists.
+    split.
+    split.
+    exists x2.
+    split.
+    congruence.
+  }
+  admit.
+  split.
+  {
+    commit.
+    do 2 dependent destruction H6.
+    eexists.
+    split.
+    split.
+    congruence.
+    exists (S n).
+    split.
+    congruence.
+
   }
 }
