Core/LogicFacts.v
@@ -5,6 +5,9 @@ From LHL Require Import
   Linearizability
   Program.
 
+From LHL.Util Require Import
+  TransUtil.
+
 From Coq Require Import
   Program.Equality
   Lists.List
@@ -26,6 +29,9 @@ Ltac pdestruct H :=
 match type of H with
 | ReltCompose ?P ?Q ?s ?ρ ?t ?σ => do 3 destruct H
 | PrecCompose ?P ?Q ?s ?ρ => do 3 destruct H
+| TIdle ?i ?s ?ρ => destruct H
+| TInvoke ?impl ?i ?Ret ?m ?s ?ρ ?t ?σ => do 2 destruct H
+| InvokeAny ?impl ?i ?s ?ρ ?t ?σ => do 2 destruct H
 | _ => fail "Cannot destruct this hypothesis"
 end.
 
@@ -36,7 +42,7 @@ repeat lazymatch goal with
 | [ H : ?P /\ ?Q |- ?G ] => destruct H
 | [ H : exists x, ?P |- ?G ] => destruct H
 | [ H : TInvoke ?impl ?i ?A ?l ?s ?ρ ?t ?σ |- ?G ] => destruct H
-| [ H : LinRw ?ρ ?σ |- ?G ] => destruct H
+| [ H : ReltToPrec ?R ?s ?ρ |- ?G ] => destruct H
 end;
 repeat lazymatch goal with
 | [ H : InterStep ?i ?st ?ev ?st' |- ?G ] => dependent destruction H
@@ -121,7 +127,7 @@ apply IHRTC.
 easy.
 Qed.
 
-Lemma precStabilizedStable {E VE F} {R : @Relt E VE F} {P} :
+Lemma precStabilizedStable {E VE F} {R : Relt E VE F} {P} :
   (R >> R ==> R) ->
   Stable R (P << R).
 intros.
@@ -133,6 +139,21 @@ exact H0.
 apply H.
 psplit.
 exact H2.
+easy.
+Qed.
+
+Lemma rtpStable {E VE F} {R} {Q : Relt E VE F} :
+  Stable R Q ->
+  Stable R (ReltToPrec Q).
+unfold Stable, stableRelt, stablePrec, ReltToPrec.
+intros.
+unfold sub, subPrec.
+intros.
+psimpl.
+exists x1, x2.
+apply H1.
+psplit.
+exact H0.
 easy.
 Qed.
 
@@ -151,7 +172,7 @@ lazymatch goal with
 | _ => idtac
 end.
 
-Lemma new_poss_refl {F} : forall (ρ : Trace (ThreadEvent F)), ρ --> ρ.
+Lemma newPossRefl {F} : forall (ρ : Trace (ThreadEvent F)), ρ --> ρ.
 intros.
 exists nil.
 split.
@@ -165,69 +186,38 @@ constructor.
 apply rt_refl.
 Qed.
 
-Lemma safeBind {E F VF VE impl i R G P A B} {m : E A} {k : A -> Prog E B} :
-  forall (QI QR S : @Relt E VE F),
-  Stable R P ->
+Lemma safeBind {E F VF VE impl i R G P A B} {S : Post E VE F B} {m : E A} {k : A -> Prog E B} :
+  forall QI QR,
   Stable R QI ->
-  Stable R QR ->
-  Stable R S ->
   Commit VF i impl R G P (CallEv m) QI ->
+  Stable R QR ->
+  (forall v,
+    Commit VF i impl R G QI (RetEv m v) QR /\
+    VerifyProg VF i impl R G QR (k v) S) ->
+  VerifyProg VF i impl R G P (Bind m k) S.
+intros.
+psimpl.
+eapply SafeBind.
+exact H.
+exact H1.
+easy.
+easy.
+Qed.
+
+(* Lemma safeBindAcc {E F VF VE impl i R G P A B} {S : Post E VE F B} {m : E A} {k : A -> Prog E B} :
+  forall QI QR,
+  Stable R QI ->
+  Commit VF i impl R G P (CallEv m) QI ->
+  Stable R QR ->
   (forall v,
     Commit VF i impl R G (P << QI) (RetEv m v) QR /\
     VerifyProg VF i impl R G (P << QI << QR) (k v) S) ->
-  VerifyProg VF i impl R G P (Bind m k) (QI >> QR >> S).
+  VerifyProg VF i impl R G P (Bind m k) S.
 intros.
-constructor.
-easy.
-intros.
-specialize (H4 v).
-split.
-split.
-apply precCompStable; easy.
-split.
-easy.
-easy.
-easy.
-Qed.
+eapply safeBind. *)
 
-Lemma safeBindUnit {E : ESig} {F VE VF impl i R G P A} {m : E unit} {k : unit -> Prog E A} :
-  forall (QI QR S : @Relt E VE F),
-  Stable R P ->
-  Stable R QI ->
-  Stable R QR ->
-  Stable R S ->
-  Commit VF i impl R G P (CallEv m) QI ->
-  Commit VF i impl R G (P << QI) (RetEv m tt) QR /\
-  VerifyProg VF i impl R G (P << QI << QR) (k tt) S ->
-  VerifyProg VF i impl R G P (Bind m k) (QI >> QR >> S).
-intros.
-apply safeBind.
-easy.
-easy.
-easy.
-easy.
-easy.
-intros.
-destruct v.
-easy.
-Qed.
-
-Lemma weakenPost {E F A i VF VE impl} {C : Prog E A} R G P Q Q' :
-  VerifyProg VF i impl R G P C Q ->
-  Stable R Q' ->
-  Q ==> Q' ->
-  VerifyProg (VE:=VE) (F:=F) VF i impl R G P C Q'.
-Admitted.
-
-Ltac bind QI QR S :=
-match goal with
-| [ |- VerifyProg ?VF ?i ?impl ?R ?G ?P (@Bind ?A ?B unit ?m ?k) ?S ] =>
-    eapply (safeBindUnit QI QR S)
-| [ |- VerifyProg ?VF ?i ?impl ?R ?G ?P (Bind ?m ?k) ?S ] =>
-    eapply (safeBind QI QR S)
-end.
 
 Theorem soundness {E F} (lay : Layer E F) VF :
   (exists R G P Q, VerifyImpl lay.(USpec) VF R G P lay.(LImpl) Q) ->
-  specRefines VF (overObj lay).
+  specRefines (overObj lay) VF.
 Admitted.
